`impl_offsets_and_sizes_are_contiguous`, `sorted`

src/Parquet/Parquet.Pulse.Jump.fst
@@ -7,6 +7,8 @@ include Parquet.Spec.Jump
 module SZ = FStar.SizeT
 module S = Pulse.Lib.Slice.Util
 module Trade = Pulse.Lib.Trade.Util
+module V = Pulse.Lib.Vec
+module PV = Parquet.Pulse.Vec
 
 inline_for_extraction
 fn impl_pred_jump_with_offset_and_size_then_parse
@@ -121,4 +123,220 @@ ensures exists* v' .
   let res = impl_pred_jump_with_offset_and_size_then_parse offset size s input v;
   Trade.trans _ _ (pts_to_serialized (serialize_filter serialize_seq_all_bytes phi) input #pm v);
   res
+}
+
+module Rel = CDDL.Pulse.Types.Base
+module I64 = FStar.Int64
+module SM = Pulse.Lib.SeqMatch.Util
+
+inline_for_extraction
+let impl_fst_f
+  (#implt: Type0)
+  (#spect: Type0)
+  (f: (spect -> (int & int)))
+  (r: Rel.rel implt spect)
+=
+    (impl: implt) ->
+    (spec: Ghost.erased spect) ->
+    stt I64.t
+      (r impl spec)
+      (fun res -> r impl spec ** pure ((I64.v res <: int) == fst (Ghost.reveal f spec)))
+
+inline_for_extraction
+let impl_snd_f
+  (#implt: Type0)
+  (#spect: Type0)
+  (f: (spect -> (int & int)))
+  (r: Rel.rel implt spect)
+=
+    (impl: implt) ->
+    (spec: Ghost.erased spect) ->
+    stt I64.t
+      (r impl spec)
+      (fun res -> r impl spec ** pure ((I64.v res <: int) == snd (Ghost.reveal f spec)))
+
+inline_for_extraction
+fn impl_offsets_and_sizes_are_contiguous
+  (#implt: Type0)
+  (#spect: Type0)
+  (f: Ghost.erased (spect -> (int & int)))
+  (r: Rel.rel implt spect)
+  (implf_fst: impl_fst_f f r)
+  (implf_snd: impl_snd_f f r)
+  (impl: PV.vec implt)
+  (#spec: Ghost.erased (list spect))
+requires
+  PV.rel_vec_of_list r impl spec
+returns res: bool
+ensures
+  PV.rel_vec_of_list r impl spec **
+  pure (res == offsets_and_sizes_are_contiguous (List.Tot.map f spec))
+{
+  unfold (PV.rel_vec_of_list r impl spec);
+  with s . assert (pts_to impl.data s);
+  SM.seq_list_match_length r s spec;
+  V.pts_to_len impl.data;
+  if (SZ.lt impl.len 2sz) {
+    fold (PV.rel_vec_of_list r impl spec);
+    true
+  } else {
+    SM.seq_list_match_cons_elim_trade _ _ _;
+    let mut pl = V.op_Array_Access impl.data 0sz;
+    let mut pres = true;
+    let mut pi = 1sz;
+    while (
+      let res = !pres;
+      if (res) {
+        SM.seq_list_match_length r _ _;
+        let i = !pi;
+        SZ.lt i impl.len
+      } else {
+        false
+      }
+    ) invariant b . exists* impll specl sr specr res i . (
+      pts_to impl.data s **
+      pts_to pl impll **
+      r impll specl **
+      SM.seq_list_match sr specr r **
+      Trade.trade
+        (r impll specl ** SM.seq_list_match sr specr r)
+        (SM.seq_list_match s spec r) **
+      pts_to pres res **
+      pts_to pi i **
+      pure (
+        SZ.v i <= Seq.length s /\
+        sr == Seq.slice s (SZ.v i) (Seq.length s) /\
+        offsets_and_sizes_are_contiguous (List.Tot.map f spec) == (res && offsets_and_sizes_are_contiguous (List.Tot.map f (specl :: specr))) /\
+        b == (res && Cons? specr)
+      )
+    ) {
+      let impl1 = !pl;
+      with spec1 . assert (r impl1 spec1);
+      let off1 = implf_fst impl1 _;
+      if (I64.lt off1 0L) {
+        pres := false
+      } else {
+        let sz1 = implf_snd impl1 _;
+        if (I64.lt sz1 0L) {
+          pres := false
+        } else {
+          SM.seq_list_match_length r _ _;
+          SM.seq_list_match_cons_elim_trade _ _ _;
+          let i = !pi;
+          with gimpl2 spec2 . assert (r impl1 spec1 ** r gimpl2 spec2);
+          let impl2 = V.op_Array_Access impl.data i;
+          rewrite each gimpl2 as impl2;
+          let off2 = implf_fst impl2 _;
+          if (I64.lt off2 off1) {
+            Trade.elim (r impl2 _ ** _) _;
+            pres := false
+          } else if (sz1 <> I64.sub off2 off1) {
+            Trade.elim (r impl2 _ ** _) _;
+            pres := false
+          } else {
+            Trade.elim_hyp_l (r impl1 _) _ _;
+            Trade.trans _ _ (SM.seq_list_match s spec r);
+            pl := impl2;
+            pi := SZ.add i 1sz;
+          }
+        }
+      }
+    };
+    Trade.elim _ _;
+    fold (PV.rel_vec_of_list r impl spec);
+    !pres
+  }
+}
+
+inline_for_extraction
+fn impl_offsets_and_sizes_are_sorted
+  (#implt: Type0)
+  (#spect: Type0)
+  (f: Ghost.erased (spect -> (int & int)))
+  (r: Rel.rel implt spect)
+  (implf_fst: impl_fst_f f r)
+  (implf_snd: impl_snd_f f r)
+  (impl: PV.vec implt)
+  (#spec: Ghost.erased (list spect))
+requires
+  PV.rel_vec_of_list r impl spec
+returns res: bool
+ensures
+  PV.rel_vec_of_list r impl spec **
+  pure (res == offsets_and_sizes_are_sorted (List.Tot.map f spec))
+{
+  unfold (PV.rel_vec_of_list r impl spec);
+  with s . assert (pts_to impl.data s);
+  SM.seq_list_match_length r s spec;
+  V.pts_to_len impl.data;
+  if (SZ.lt impl.len 2sz) {
+    fold (PV.rel_vec_of_list r impl spec);
+    true
+  } else {
+    SM.seq_list_match_cons_elim_trade _ _ _;
+    let mut pl = V.op_Array_Access impl.data 0sz;
+    let mut pres = true;
+    let mut pi = 1sz;
+    while (
+      let res = !pres;
+      if (res) {
+        SM.seq_list_match_length r _ _;
+        let i = !pi;
+        SZ.lt i impl.len
+      } else {
+        false
+      }
+    ) invariant b . exists* impll specl sr specr res i . (
+      pts_to impl.data s **
+      pts_to pl impll **
+      r impll specl **
+      SM.seq_list_match sr specr r **
+      Trade.trade
+        (r impll specl ** SM.seq_list_match sr specr r)
+        (SM.seq_list_match s spec r) **
+      pts_to pres res **
+      pts_to pi i **
+      pure (
+        SZ.v i <= Seq.length s /\
+        sr == Seq.slice s (SZ.v i) (Seq.length s) /\
+        offsets_and_sizes_are_sorted (List.Tot.map f spec) == (res && offsets_and_sizes_are_sorted (List.Tot.map f (specl :: specr))) /\
+        b == (res && Cons? specr)
+      )
+    ) {
+      let impl1 = !pl;
+      with spec1 . assert (r impl1 spec1);
+      let off1 = implf_fst impl1 _;
+      if (I64.lt off1 0L) {
+        pres := false
+      } else {
+        let sz1 = implf_snd impl1 _;
+        if (I64.lt sz1 0L) {
+          pres := false
+        } else {
+          SM.seq_list_match_length r _ _;
+          SM.seq_list_match_cons_elim_trade _ _ _;
+          let i = !pi;
+          with gimpl2 spec2 . assert (r impl1 spec1 ** r gimpl2 spec2);
+          let impl2 = V.op_Array_Access impl.data i;
+          rewrite each gimpl2 as impl2;
+          let off2 = implf_fst impl2 _;
+          if (I64.lt off2 off1) {
+            Trade.elim (r impl2 _ ** _) _;
+            pres := false
+          } else if (I64.gt sz1 (I64.sub off2 off1)) {
+            Trade.elim (r impl2 _ ** _) _;
+            pres := false
+          } else {
+            Trade.elim_hyp_l (r impl1 _) _ _;
+            Trade.trans _ _ (SM.seq_list_match s spec r);
+            pl := impl2;
+            pi := SZ.add i 1sz;
+          }
+        }
+      }
+    };
+    Trade.elim _ _;
+    fold (PV.rel_vec_of_list r impl spec);
+    !pres
+  }
 }
